Added read of a component's local buffer by another in the events
Made changes necessary to include the value read in the event.
Had to add an EqType for the values to allow comparison between events
now that a value is part of it.

This would also allow to have pointers returned or passed as argument in
the events only (it could only take integers before).

Plus, with the imports of ssrnat and eqtype, it is not even necessary to
have Pointer.eq since the equality of pointers ( (nat * nat) * Z) is
already inferred (nat and Z already have EqTypes)

Common/Values.v
@@ -1,5 +1,8 @@
 Require Import Common.Definitions.
 Require Import Common.Util.
+Require Import Lib.Extra.
+From mathcomp Require Import
+     ssreflect ssrnat eqtype.
 
 Module Block.
   Definition id := nat.
@@ -18,11 +21,6 @@ Module Pointer.
 
   Definition offset (p : t) : Block.offset :=
     let '(_, _, o) := p in o.
-
-  Definition eq (p1 p2 : t) : bool :=
-    let '(C1, b1, o1) := p1 in
-    let '(C2, b2, o2) := p2 in
-    (Nat.eqb C1 C2) && (Nat.eqb b1 b2) && (Z.eqb o1 o2).
 
   Definition leq (p1 p2 : t) : option bool :=
     let '(C1, b1, o1) := p1 in
@@ -78,6 +76,28 @@ Inductive value : Type :=
 | Ptr : Pointer.t -> value
 | Undef : value.
 
+Definition eqvalue v1 v2 :=
+  match v1, v2 with
+  | Int z1, Int z2 => z1 == z2
+  | Ptr p1, Ptr p2 =>  p1 == p2
+  | Undef, Undef => true         (* should undef not be equal to itself ? Since it can be anything *)
+  | _, _ => false
+  end.
+
+Lemma eqvalueP : Equality.axiom eqvalue.
+Proof.
+  move; elim => [z1 | p1 |] [z2 | p2|]//= ;
+                 apply: (iffP idP); move => H; inversion H ; try constructor.
+  by move: H => /Z.eqb_spec => H; rewrite H.
+  done.
+  by move: H => /pair_eqP => H; rewrite H.
+  done.
+Qed.
+
+Definition value_eqMixin: Equality.mixin_of value := EqMixin eqvalueP.
+Canonical value_eqType := Eval hnf in EqType value value_eqMixin.
+
+
 Inductive binop := Add | Minus | Mul | Eq | Leq.
 
 Definition eval_binop (op : binop) (v1 v2 : value) : value :=
@@ -98,7 +118,7 @@ Definition eval_binop (op : binop) (v1 v2 : value) : value :=
                              else
                                Undef
   | Minus, Ptr p,  Int n  => Ptr (Pointer.sub p n)
-  | Eq,    Ptr p1, Ptr p2 => Int (Util.Z.of_bool (Pointer.eq p1 p2))
+  | Eq,    Ptr p1, Ptr p2 => Int (Util.Z.of_bool (p1 == p2))
   | Leq,   Ptr p1, Ptr p2 => match Pointer.leq p1 p2 with
                              | Some res => Int (Util.Z.of_bool res)
                              | None     => Undef
